src/Narcissus/Common/ComposeOpt.v
@@ -189,50 +189,16 @@ Proof.
       simpl in *; try discriminate.
     eapply (proj2 decode1_pf) in Heqo; eauto.
     destruct Heqo as [? [? ?] ].
-    apply unfold_computes in H1; intuition; simpl in *;
+    rewrite unfold_computes in H1; intuition; simpl in *;
       destruct_ex; intuition; subst.
     eapply (proj2 (decode2_pf _)) in H0; eauto.
     destruct H0 as [? ?]; destruct_ex; intuition; subst.
-    unfold RestrictFormat in H1; apply unfold_computes in H1; intuition.
+    unfold RestrictFormat in H1; rewrite unfold_computes in H1; intuition.
     rewrite H5.
     unfold compose; eexists; intuition eauto.
     repeat first [computes_to_econstructor
                   | apply unfold_computes; eauto ]. }
 Qed.
-
-Lemma compose_format_correct_simpl'
-      {A A' B}
-      {cache : Cache}
-      {monoid : Monoid B}
-      (project : A -> A')
-      (format1 : FormatM A' B)
-      (format2 : FormatM A B)
-      (decode1 : DecodeM (A' * B) B)
-      (*oblivious_decoder : forall bs data env bs' env',
-          decode1 bs env = Some (data, bs', env') ->
-          forall bs'', decode1 (mappend bs bs'') env = Some (data, mappend bs' bs'', env')*)
-      (decode1_pf : CorrectDecoder_simpl
-                      (fun data_rest env binxenv =>
-                         exists bin', fst binxenv = mappend bin' (snd data_rest) /\
-                                      format1 (fst data_rest) env (bin', snd binxenv))
-                      decode1)
-      (decode2 : A' -> B -> CacheDecode -> option (A * CacheDecode))
-      (decode2_pf : forall proj,
-          CorrectDecoder_simpl (RestrictFormat format2 (fun data => project data = proj))
-                               (decode2 proj))
-  : CorrectDecoder_simpl
-      (fun (data : A) (ctx : CacheFormat) =>
-         compose _ (format1 (project data)) (format2 data) ctx
-      )%comp
-      (fun (bin : B) (env : CacheDecode) =>
-         `(proj, env') <- decode1 bin env;
-           decode2 (fst proj) (snd proj) env').
-Proof.
-  eapply CorrectDecoder_simpl_equiv_format; eauto.
-  eapply CorrectDecoder_simpl_equiv_decode; try eassumption.
-  eapply CorrectDecoder_simpl_no_inv.
-  eapply CorrectDecoder_simpl_strict_equiv.
-Abort.
 
 (* For decoding fixed fields that do no depend on the object *)
 (* being formatd, e.g. version numbers in an IP packet. This *)
